Use an env

src/defs/statics.lean
@@ -1,59 +1,68 @@
 import defs.syntax
 
+structure env :=
+  (exps: cx typ)
+
+def env.insert_exp (Γ: env) (x: var) (τ: typ): env :=
+  {exps := cx.insert Γ.exps x τ, ..Γ}
+
+def env.lookup_exp (Γ: env) (x: var) (τ: typ): Prop :=
+  cx.lookup Γ.exps x τ
+
 -- Γ ⊢ e : τ
-inductive has_typ: cx typ -> exp -> typ -> Prop
-| int {Γ: cx typ} {n: ℤ}: has_typ Γ (exp.int n) typ.int
-| true {Γ: cx typ}: has_typ Γ exp.true typ.bool
-| false {Γ: cx typ}: has_typ Γ exp.false typ.bool
+inductive has_typ: env -> exp -> typ -> Prop
+| int {Γ: env} {n: ℤ}: has_typ Γ (exp.int n) typ.int
+| true {Γ: env}: has_typ Γ exp.true typ.bool
+| false {Γ: env}: has_typ Γ exp.false typ.bool
 | if_
-    {Γ: cx typ}
+    {Γ: env}
     {e1 e2 e3: exp} {τ: typ}:
     has_typ Γ e1 typ.bool ->
     has_typ Γ e2 τ ->
     has_typ Γ e3 τ ->
     has_typ Γ (exp.if_ e1 e2 e3) τ
 | var
-    {Γ: cx typ} {x: var} {τ: typ}:
-    cx.lookup Γ x τ ->
+    {Γ: env} {x: var} {τ: typ}:
+    env.lookup_exp Γ x τ ->
     has_typ Γ (exp.var x) τ
 | fn
-    {Γ: cx typ} {x: var} {τ1 τ2: typ} {e: exp}:
-    has_typ (cx.insert Γ x τ1) e τ2 ->
+    {Γ: env} {x: var} {τ1 τ2: typ} {e: exp}:
+    has_typ (env.insert_exp Γ x τ1) e τ2 ->
     has_typ Γ (exp.fn x τ1 e) (typ.arrow τ1 τ2)
 | app
-    {Γ: cx typ} {e1 e2: exp} {τ1 τ2: typ}:
+    {Γ: env} {e1 e2: exp} {τ1 τ2: typ}:
     has_typ Γ e1 (typ.arrow τ1 τ2) ->
     has_typ Γ e2 τ1 ->
     has_typ Γ (exp.app e1 e2) τ2
-| unit {Γ: cx typ}: has_typ Γ exp.unit typ.unit
+| unit {Γ: env}: has_typ Γ exp.unit typ.unit
 | pair
-    {Γ: cx typ} {e1 e2: exp} {τ1 τ2: typ}:
+    {Γ: env} {e1 e2: exp} {τ1 τ2: typ}:
     has_typ Γ e1 τ1 ->
     has_typ Γ e2 τ2 ->
     has_typ Γ (exp.pair e1 e2) (typ.pair τ1 τ2)
 | pair_left
-    {Γ: cx typ} {e: exp} {τ1 τ2: typ}:
+    {Γ: env} {e: exp} {τ1 τ2: typ}:
     has_typ Γ e (typ.pair τ1 τ2) ->
     has_typ Γ (exp.pair_left e) τ1
 | pair_right
-    {Γ: cx typ} {e: exp} {τ1 τ2: typ}:
+    {Γ: env} {e: exp} {τ1 τ2: typ}:
     has_typ Γ e (typ.pair τ1 τ2) ->
     has_typ Γ (exp.pair_right e) τ2
 | either_left
-    {Γ: cx typ} {e: exp} {τ1 τ2: typ}:
+    {Γ: env} {e: exp} {τ1 τ2: typ}:
     has_typ Γ e τ1 ->
     has_typ Γ (exp.either_left τ2 e) (typ.either τ1 τ2)
 | either_right
-    {Γ: cx typ} {e: exp} {τ1 τ2: typ}:
+    {Γ: env} {e: exp} {τ1 τ2: typ}:
     has_typ Γ e τ2 ->
     has_typ Γ (exp.either_right τ1 e) (typ.either τ1 τ2)
 | case_never
-    {Γ: cx typ} {e: exp} {τ: typ}:
+    {Γ: env} {e: exp} {τ: typ}:
     has_typ Γ e typ.never ->
     has_typ Γ (exp.case_never τ e) τ
 | case
-    {Γ: cx typ} {eh e1 e2: exp} {x1 x2: var} {τ1 τ2 τ: typ}:
+    {Γ: env} {eh e1 e2: exp} {x1 x2: var} {τ1 τ2 τ: typ}:
     has_typ Γ eh (typ.either τ1 τ2) ->
-    has_typ (cx.insert Γ x1 τ1) e1 τ ->
-    has_typ (cx.insert Γ x2 τ2) e2 τ ->
+    has_typ (env.insert_exp Γ x1 τ1) e1 τ ->
+    has_typ (env.insert_exp Γ x2 τ2) e2 τ ->
     has_typ Γ (exp.case eh x1 e1 x2 e2) τ
