src/lemmas/inversion.lean
@@ -1,7 +1,7 @@
 import defs.statics
 
 theorem inversion_if
-  {Γ: cx typ} {e1 e2 e3: exp} {τ: typ}
+  {Γ: env} {e1 e2 e3: exp} {τ: typ}
   (et: has_typ Γ (exp.if_ e1 e2 e3) τ)
   : has_typ Γ e1 typ.bool ∧ has_typ Γ e2 τ ∧ has_typ Γ e3 τ :=
 begin
@@ -14,7 +14,7 @@ begin
 end
 
 theorem inversion_app
-  {Γ: cx typ} {e1 e2: exp} {τ2: typ}
+  {Γ: env} {e1 e2: exp} {τ2: typ}
   (et: has_typ Γ (exp.app e1 e2) τ2)
   : ∃ (τ1: typ), has_typ Γ e1 (typ.arrow τ1 τ2) ∧ has_typ Γ e2 τ1 :=
 begin
@@ -26,9 +26,9 @@ begin
 end
 
 theorem inversion_fn
-  {Γ: cx typ} {x: var} {τ1 τ: typ} {e: exp}
+  {Γ: env} {x: var} {τ1 τ: typ} {e: exp}
   (et: has_typ Γ (exp.fn x τ1 e) τ)
-  : ∃ (τ2: typ), τ = typ.arrow τ1 τ2 ∧ has_typ (cx.insert Γ x τ1) e τ2 :=
+  : ∃ (τ2: typ), τ = typ.arrow τ1 τ2 ∧ has_typ (env.insert_exp Γ x τ1) e τ2 :=
 begin
   cases et,
   existsi et_τ2,
@@ -38,7 +38,7 @@ begin
 end
 
 theorem inversion_prod
-  {Γ: cx typ} {e1 e2: exp} {τ: typ}
+  {Γ: env} {e1 e2: exp} {τ: typ}
   (et: has_typ Γ (exp.pair e1 e2) τ)
   : ∃ (τ1 τ2: typ), τ = (typ.pair τ1 τ2) ∧ has_typ Γ e1 τ1 ∧ has_typ Γ e2 τ2 :=
 begin
@@ -52,7 +52,7 @@ begin
 end
 
 theorem inversion_prod_left
-  {Γ: cx typ} {e: exp} {τ1: typ}
+  {Γ: env} {e: exp} {τ1: typ}
   (et: has_typ Γ (exp.pair_left e) τ1)
   : ∃ (τ2: typ), has_typ Γ e (typ.pair τ1 τ2) :=
 begin
@@ -62,7 +62,7 @@ begin
 end
 
 theorem inversion_prod_right
-  {Γ: cx typ} {e: exp} {τ2: typ}
+  {Γ: env} {e: exp} {τ2: typ}
   (et: has_typ Γ (exp.pair_right e) τ2)
   : ∃ (τ1: typ), has_typ Γ e (typ.pair τ1 τ2) :=
 begin
@@ -72,7 +72,7 @@ begin
 end
 
 theorem inversion_sum_left
-  {Γ: cx typ} {e: exp} {τ2 τ: typ}
+  {Γ: env} {e: exp} {τ2 τ: typ}
   (et: has_typ Γ (exp.either_left τ2 e) τ)
   : ∃ (τ1: typ), τ = typ.either τ1 τ2 ∧ has_typ Γ e τ1 :=
 begin
@@ -84,7 +84,7 @@ begin
 end
 
 theorem inversion_sum_right
-  {Γ: cx typ} {e: exp} {τ1 τ: typ}
+  {Γ: env} {e: exp} {τ1 τ: typ}
   (et: has_typ Γ (exp.either_right τ1 e) τ)
   : ∃ (τ2: typ), τ = typ.either τ1 τ2 ∧ has_typ Γ e τ2 :=
 begin
@@ -96,7 +96,7 @@ begin
 end
 
 theorem inversion_case_never
-  {Γ: cx typ} {e: exp} {τ τ': typ}
+  {Γ: env} {e: exp} {τ τ': typ}
   (et: has_typ Γ (exp.case_never τ e) τ')
   : τ = τ' ∧ has_typ Γ e typ.never :=
 begin
@@ -107,12 +107,12 @@ begin
 end
 
 theorem inversion_case
-  {Γ: cx typ} {eh e1 e2: exp} {x1 x2: var} {τ: typ}
+  {Γ: env} {eh e1 e2: exp} {x1 x2: var} {τ: typ}
   (et: has_typ Γ (exp.case eh x1 e1 x2 e2) τ)
   : ∃ (τ1 τ2: typ),
     has_typ Γ eh (typ.either τ1 τ2) ∧
-    has_typ (cx.insert Γ x1 τ1) e1 τ ∧
-    has_typ (cx.insert Γ x2 τ2) e2 τ :=
+    has_typ (env.insert_exp Γ x1 τ1) e1 τ ∧
+    has_typ (env.insert_exp Γ x2 τ2) e2 τ :=
 begin
   cases et,
   existsi [et_τ1, et_τ2],
